simplify
git-svn-id: https://projects.brucker.ch/hol-testgen/svn/HOL-TestGen/trunk/hol-testgen@13758 3260e6d1-4efc-4170-b0a7-36055960796d

C11-FrontEnd/examples/C_paper.thy
@@ -75,77 +75,24 @@ fun command0 dir name =
                        \in " ^ hook ^ " (stack |> hd |> map_svalue0 MlyValue.reduce" ^ Int.toString rule ^ ") env_lang end context")
                     (ML_Lex.read_source false src)
                 end)))
-
-fun command dir name =
-  C_Annotation.command' name ""
-    (fn (stack1, (to_delay, stack2)) =>
-      C_Parse.range C_Parse.ML_source >>
-        (fn (src, range) =>
-          (fn f => Once ((stack1, stack2), (range, dir, to_delay, f)))
-            (fn NONE =>
-                let val setup = "setup"
-                in expression
-                    (Input.range_of src)
-                    setup
-                    "stack_data -> stack_data_elem -> C_Env.env_lang -> Context.generic -> Context.generic"
-                    ("fn context => \
-                       \let val (stack, env_lang) = Stack_Data_Lang.get context \
-                       \in " ^ setup ^ " stack (stack |> hd) env_lang end context")
-                    (ML_Lex.read_source false src) end
-              | SOME rule => 
-                let val hook = "hook"
-                in expression
-                    (Input.range_of src)
-                    hook
-                    ("stack_data -> " ^ MlyValue.type_reduce rule ^ " stack_elem -> C_Env.env_lang -> Context.generic -> Context.generic")
-                    ("fn context => \
-                       \let val (stack, env_lang) = Stack_Data_Lang.get context \
-                       \in " ^ hook ^ " stack (stack |> hd |> map_svalue0 MlyValue.reduce" ^ Int.toString rule ^ ") env_lang end context")
-                    (ML_Lex.read_source false src)
-                end)))
-
 in
 val _ = Theory.setup (   command0 Bottom_up ("ML_setup", \<^here>)
                       #> command0 Top_down ("ML_setup\<Down>", \<^here>))
-val _ = Theory.setup (   command Bottom_up ("ML\<Up>", \<^here>)
-                      #> command Bottom_up ("setup1", \<^here>)
-                      #> command Top_down ("setup1_rev", \<^here>)
-                      #> command Top_down ("ML\<Down>", \<^here>))
 end
-\<close>
-
-ML\<open>
-fun show_env0 make_string f msg context =
-  warning ("(" ^ msg ^ ") "
-           ^ make_string (f (the (Symtab.lookup (#tab (C11_core.Data.get context))
-                                                (Context.theory_name (Context.theory_of context))))))
-
-val show_env = tap o show_env0 @{make_string} length
 
 val C' = C_Outer_Syntax.C' (fn _ => fn _ => fn pos =>
                              tap (fn _ => warning ("Parser: No matching grammar rule " ^ Position.here pos)))
-\<close>
 
-
-ML\<open>
-fun command_c' name _ _ =
+fun C_define dir name _ _ =
   Context.map_theory 
     (C_Annotation.command' name ""
       (fn (stack1, (to_delay, stack2)) =>
         C_Parse.range C_Parse.ML_source >>
           (fn (src, range) =>
-            (fn f => Once ((stack1, stack2), (range, Bottom_up, to_delay, f)))
+            (fn f => Once ((stack1, stack2), (range, dir, to_delay, f)))
               (fn _ => fn context => C' (Stack_Data_Lang.get context |> #2) src context))))
 
-fun command_c'' name _ _ =
-  Context.map_theory 
-    (C_Annotation.command' name ""
-      (fn (stack1, (to_delay, stack2)) =>
-        C_Parse.range C_Parse.ML_source >>
-          (fn (src, range) =>
-            (fn f => Once ((stack1, stack2), (range, Top_down, to_delay, f)))
-              (fn _ => fn context => C' (Stack_Data_Lang.get context |> #2) src context))))
-
+local
 fun fun_decl a v s ctxt =
   let
     val (b, ctxt') = ML_Context.variant a ctxt;
@@ -153,35 +100,27 @@ fun fun_decl a v s ctxt =
     val body = ML_Context.struct_name ctxt ^ "." ^ b;
     fun decl (_: Proof.context) = (env, body);
   in (decl, ctxt') end;
-
+in
 val _ = Theory.setup
-  (ML_Antiquotation.declaration (Binding.make ("C_define", \<^here>)) (Scan.lift (Parse.sym_ident
- -- Parse.position Parse.name))
+  (ML_Antiquotation.declaration
+    @{binding "C_define"}
+    (Scan.lift (Parse.sym_ident -- Parse.position Parse.name))
     (fn _ => fn (top_down, (name, pos)) =>
       tap (fn ctxt => Context_Position.reports ctxt [(pos, Markup.keyword1)]) #>
-      fun_decl "cmd" "x" ((case top_down of "\<Up>" => "command_c'" | "\<Down>" => "command_c''" | _ => error "Illegal symbol") ^ " (\"" ^ name ^ "\", " ^ ML_Syntax.print_position pos ^ ")")))
+      fun_decl "cmd" "x" ( "C_define "
+                         ^ (case top_down of "\<Up>" => "Bottom_up"
+                                           | "\<Down>" => "Top_down"
+                                           | _ => error "Illegal symbol")
+                         ^ " (\"" ^ name ^ "\", " ^ ML_Syntax.print_position pos ^ ")")))
+end
 
 fun C opt = case opt of NONE => (fn src => tap (fn _ => C_Outer_Syntax.C src))
                       | SOME env => C' env
+
+fun highlight (_, (_, pos1, pos2)) =
+  tap (fn _ => Position.reports_text [((Position.range (pos1, pos2)
+                                        |> Position.range_position, Markup.intensify), "")])
 \<close>
-
-ML\<open>
-fun print_top make_string (_, (value, pos1, pos2)) thy =
-  let
-    val () = writeln (make_string value)
-    val () = Position.reports_text [((Position.range (pos1, pos2) 
-                                    |> Position.range_position, Markup.intensify), "")]
-  in thy end
-
-fun highlight (_, (_, pos1, pos2)) thy =
-  let
-    val () = Position.reports_text [((Position.range (pos1, pos2) 
-                                    |> Position.range_position, Markup.intensify), "")]
-  in thy end
-\<close>
-
-setup \<open>ML_Antiquotation.inline @{binding highlight}
-                               (Args.context >> K ("highlight " ^ " "))\<close>
 
 C (*NONE*) \<comment> \<open> the command starts with a default empty environment \<close>
 \<open>int f (int a)
