C11-FrontEnd/src/C_Annotation.thy
@@ -975,38 +975,69 @@ fun expression range name constraint body ants context = context |>
       ML_Lex.read (": " ^ constraint ^ " =") @ ants @
       ML_Lex.read ("in " ^ body ^ " end (Context.the_generic_context ())));")) end;
 
-fun command dir name =
+structure C_Toplevel =
+struct
+val theory = Context.map_theory
+val generic_theory = I
+end
+
+structure Isar_Cmd0 = 
+struct
+fun ML source =  ML_Context.exec (fn () =>
+                    ML_Context.eval_source (ML_Compiler.verbose true ML_Compiler.flags) source) #>
+                  Local_Theory.propagate_ml_env
+end
+
+structure C_Isar_Cmd = 
+struct
+fun setup src =
+ fn NONE =>
+    let val setup = "setup"
+    in expression
+        (Input.range_of src)
+        setup
+        "stack_data -> stack_data_elem -> C_Env.env_lang -> Context.generic -> Context.generic"
+        ("fn context => \
+           \let val (stack, env_lang) = Stack_Data_Lang.get context \
+           \in " ^ setup ^ " stack (stack |> hd) env_lang end context")
+        (ML_Lex.read_source false src) end
+  | SOME rule => 
+    let val hook = "hook"
+    in expression
+        (Input.range_of src)
+        hook
+        ("stack_data -> " ^ MlyValue.type_reduce rule ^ " stack_elem -> C_Env.env_lang -> Context.generic -> Context.generic")
+        ("fn context => \
+           \let val (stack, env_lang) = Stack_Data_Lang.get context \
+           \in " ^ hook ^ " stack (stack |> hd |> map_svalue0 MlyValue.reduce" ^ Int.toString rule ^ ") env_lang end context")
+        (ML_Lex.read_source false src)
+    end
+
+end
+
+fun command0 f dir name =
   C_Annotation.command' name ""
     (fn (stack1, (to_delay, stack2)) =>
       C_Parse.range C_Parse.ML_source >>
         (fn (src, range) =>
-          (fn f => Once ((stack1, stack2), (range, dir, to_delay, f)))
-            (fn NONE =>
-                let val setup = "setup"
-                in expression
-                    (Input.range_of src)
-                    setup
-                    "stack_data -> stack_data_elem -> C_Env.env_lang -> Context.generic -> Context.generic"
-                    ("fn context => \
-                       \let val (stack, env_lang) = Stack_Data_Lang.get context \
-                       \in " ^ setup ^ " stack (stack |> hd) env_lang end context")
-                    (ML_Lex.read_source false src) end
-              | SOME rule => 
-                let val hook = "hook"
-                in expression
-                    (Input.range_of src)
-                    hook
-                    ("stack_data -> " ^ MlyValue.type_reduce rule ^ " stack_elem -> C_Env.env_lang -> Context.generic -> Context.generic")
-                    ("fn context => \
-                       \let val (stack, env_lang) = Stack_Data_Lang.get context \
-                       \in " ^ hook ^ " stack (stack |> hd |> map_svalue0 MlyValue.reduce" ^ Int.toString rule ^ ") env_lang end context")
-                    (ML_Lex.read_source false src)
-                end)))
+          Once ((stack1, stack2), (range, dir, to_delay, K (f src)))))
+
+fun command f dir name =
+  C_Annotation.command' name ""
+    (fn (stack1, (to_delay, stack2)) =>
+      C_Parse.range C_Parse.ML_source >>
+        (fn (src, range) =>
+          Once ((stack1, stack2), (range, dir, to_delay, f src))))
 
 in
-val _ = Theory.setup (   command Bottom_up ("ML", \<^here>)
-                      #> command Top_down ("ML_reverse", \<^here>))
+val _ = Theory.setup (   command (C_Toplevel.generic_theory oo C_Isar_Cmd.setup) Bottom_up ("\<approx>setup", \<^here>)
+                      #> command (C_Toplevel.generic_theory oo C_Isar_Cmd.setup) Top_down ("\<approx>setup\<Down>", \<^here>)
+                      #> command0 (C_Toplevel.theory o Isar_Cmd.setup) Bottom_up ("setup", \<^here>)
+                      #> command0 (C_Toplevel.theory o Isar_Cmd.setup) Top_down ("setup\<Down>", \<^here>)
+                      #> command0 (C_Toplevel.generic_theory o Isar_Cmd0.ML) Bottom_up ("ML", \<^here>)
+                      #> command0 (C_Toplevel.generic_theory o Isar_Cmd0.ML) Top_down ("ML\<Down>", \<^here>))
 end
+
 \<close>
 
 end
